\documentclass[twoside]{article}

\input{./../../preamble.tex}
\title{Analysis II HW 6}

\begin{document}
    \maketitle

    \exercise{1}
    We will first prove that $\cos \frac{\pi}{2} = 0$.
    \begin{proof}
        Using the angle summation identity for $\cos$ we get that 
        \begin{equation*}
            \cos(\frac{\pi}{2}) = \cos(\pi - \frac{\pi}{2})
            = \cos \pi \cos \frac{\pi}{2} - \sin \pi \sin \frac{\pi}{2}
            = \cos \pi \cos \frac{\pi}{2}.
        \end{equation*}
        Rearranging,
        \begin{equation*}
            \cos \frac{\pi}{2} (\cos \pi) + 1 = 0,
        \end{equation*}
        therefore,
        \begin{equation*}
            \cos \frac{\pi}{2} = 0 \quad \text{and} \quad \cos \pi = -1.
        \end{equation*}
    \end{proof}

    Now, we prove that $\cos x > 0, x \in [0, \frac{\pi}{2})$.
    \begin{proof}
        As shown in class, $(\cos x)^{\prime} = -\sin x < 0, x \in [0, \pi)$.
        Therefore, $\cos x$ is strictly decresing on $(0, \pi)$.
        However, as shown before, $\cos \frac{\pi}{2} = 0$, so it must be the case that 
        $\cos x > 0, x \in [0, \frac{\pi}{2})$.
    \end{proof}

    \exercise{2}
    \subexercise{a}
    We start by noting that if we take $\sin^{2} x + \cos^{2} x = 1$ and divide by 
    $\cos^{2}x$ on both sides we get $\tan^{2} x + 1 = \sec^{2} x$.

    Now, using the quotient rule
    \begin{align*}
        \dv{}{x}\tan x
        &= \dv{}{x} \frac{\sin x}{\cos x},\\ 
        &= \frac{\cos^{2} x + \sin^{2} x}{\cos^{2} x},\\ 
        &= \sec^{2}x = 1 + \tan^{2} x,
    \end{align*}
    as needed.

    \subexercise{b}
    Since $\sin x$ is continuous everywhere and $\cos x = 0$ only when $x = \pm \frac{\pi}{2}$,
    and also continuous everywhere, we get that $\tan x$ is continuous in the interval.

    Now, since $(\tan x)^{\prime} = 1 + \tan^{2} x \geq 1$ for all $x \in (-\frac{\pi}{2}, \frac{\pi}{2})$,
    it is also increasing in the interval.

    \subexercise{c}
    By the Inverse Function Thm. we have that
    \begin{equation*}
        (\arctan x)^{\prime} = \frac{1}{1 + (\tan \arctan x)^{2}} = \frac{1}{1 + x^{2}}
    \end{equation*}

    Then taking the derivative of the other side,
    \begin{equation*}
        \dv{}{x} \sum_{n = 0}^{\infty} \frac{(-1)^{n}x^{2n + 1}}{(2n + 1)}
        = \sum_{n = 0}^{\infty} (-1)^{n} x^{2n} = \frac{1}{1 + x^{2}}.
    \end{equation*}
    Therefore, by the uniqueness of power series,
    \begin{equation*}
        \dv{}{x} \arctan x = \dv{}{x} \sum_{n = 0}^{\infty} \frac{(-1)^{n}x^{2n + 1}}{(2n + 1)}
    \end{equation*}
    and
    \begin{equation*}
         \arctan x = \sum_{n = 0}^{\infty} \frac{(-1)^{n}x^{2n + 1}}{(2n + 1)}
    \end{equation*}

    \exercise{3}

    \exercise{4}
    \begin{proof}
        Let $\sum_{i, j} \abs{a_{i,j}}$ converge. Now, let $b_{i,j} = \max(a_{i,j}, 0)$ and
        $c_{i,j} = \max(-a_{i,j}, 0)$. We now have that 
        $0 \leq b_{i,j} \leq \abs{a_{i,j}}$ and $0 \leq c_{i,j} \leq \abs{a_{i,j}}$.
        Therefore, $\sum_{i,j} b_{i,j}, \sum_{i,j} c_{i,j}$ converge (using the comparison test).

        This now implies that 
        \begin{equation*}
        \sum_{i,j} b_{i,j} - \sum_{i,j} c_{i,j} = \sum_{i,j} b_{i,j} - c_{i,j}
        = \sum_{i,j} a_{i,j}
        \end{equation*}
        converges. We can combine the sums because the summations are finite (they converge).
    \end{proof}

    
\end{document}
